RocqOfRust/revm/revm_interpreter/instructions/simulate/host/extcodecopy.v
@@ -4,21 +4,30 @@ Require Import alloy_primitives.bytes.simulate.mod.
 Require Import alloy_primitives.links.aliases.
 Require Import bytes.simulate.bytes.
 Require Import core.links.array.
+Require Import core.links.result.
 Require Import core.num.simulate.mod.
+Require Import core.simulate.option.
 Require Import core.simulate.cmp.
 Require Import revm.revm_context_interface.links.host.
 Require Import revm.revm_context_interface.links.journaled_state.
 Require Import revm.revm_context_interface.simulate.host.
 Require Import revm.revm_context_interface.simulate.journaled_state.
 Require Import revm.revm_interpreter.gas.simulate.calc.
+Require Import revm.revm_interpreter.gas.simulate.constants.
 Require Import revm.revm_interpreter.instructions.links.host.extcodecopy.
 Require Import revm.revm_interpreter.instructions.simulate.macros.
 Require Import revm.revm_interpreter.instructions.simulate.utility.
 Require Import revm.revm_interpreter.links.instruction_context.
+Require Import revm.revm_interpreter.links.gas.
 Require Import revm.revm_interpreter.links.interpreter.
 Require Import revm.revm_interpreter.links.instruction_result.
 Require Import revm.revm_interpreter.links.interpreter_types.
+Require Import revm.revm_interpreter.simulate.gas.
+Require Import revm.revm_interpreter.simulate.interpreter.
 Require Import revm.revm_interpreter.simulate.interpreter_types.
+Require Import revm.revm_primitives.links.hardfork.
+Require Import revm.revm_primitives.simulate.hardfork.
+Require Import revm.revm_bytecode.links.bytecode.
 Require Import ruint.simulate.lib.
 
 Definition extcodecopy
@@ -33,43 +42,74 @@ Definition extcodecopy
   popn_macro interpreter 4 (fun interpreter => (interpreter, host)) (fun arr interpreter =>
   let '⟬ address; memory_offset; code_offset; len_u256 ⟭ := arr.(array.value) in
   let address := Impl_IntoAddress_for_U256.into_address address in
-  let '(code_opt, host) := IHost.(Host.code) host address in
-  match code_opt with
-  | None =>
-    let control :=
-      IInterpreterTypes.(InterpreterTypes.LoopControl_for_Control).(LoopControl.set_instruction_result)
-        interpreter.(Interpreter.control)
-        instruction_result.InstructionResult.FatalExternalError in
-    (interpreter <| Interpreter.control := control |>, host)
-  | Some code =>
-
-  as_usize_or_fail_ret_macro interpreter len_u256 None
-    (fun interpreter => (interpreter, host)) (fun len interpreter =>
-  let '(code, load) := Impl_Eip7702CodeLoad.into_components code in
   let spec_id :=
     IInterpreterTypes.(InterpreterTypes.RuntimeFlag_for_RuntimeFlag).(RuntimeFlag.spec_id)
       interpreter.(Interpreter.runtime_flag) in
-  gas_or_fail_macro interpreter (calc.extcodecopy_cost spec_id len load)
+  as_usize_or_fail_ret_macro interpreter len_u256 None
+    (fun interpreter => (interpreter, host)) (fun len interpreter =>
+  let copy_cost :=
+    match calc.copy_cost 0 len with
+    | Some gas => gas
+    | None => Impl_u64.MAX
+    end in
+  gas_macro interpreter copy_cost
     (fun interpreter => (interpreter, host)) (fun interpreter =>
-  if i[len] =? 0 then
-    (interpreter, host)
-  else
-  as_usize_or_fail_ret_macro interpreter memory_offset None
-    (fun interpreter => (interpreter, host)) (fun memory_offset interpreter =>
+  let memory_offset_usize := {| Integer.value := 0 |} in
+  let '(memory_offset_usize, interpreter) :=
+    if i[len] =? 0 then
+      (memory_offset_usize, interpreter)
+    else
+      as_usize_or_fail_ret_macro interpreter memory_offset None
+      (fun interpreter => (memory_offset_usize, interpreter)) (fun memory_offset interpreter =>
+      resize_memory_macro interpreter memory_offset len
+        (fun interpreter => (memory_offset, interpreter)) (fun interpreter =>
+      (memory_offset, interpreter))) in
+  let get_code interpreter host :=
+    if Impl_SpecId.is_enabled_in spec_id SpecId.BERLIN then
+      gas_macro interpreter WARM_STORAGE_READ_COST
+        (fun interpreter => (None, interpreter, host)) (fun interpreter =>
+      let skip_cold_load :=
+        interpreter.(Interpreter.gas).(Gas.remaining).(Integer.value) <?
+        COLD_ACCOUNT_ACCESS_COST_ADDITIONAL.(Integer.value) in
+      let '(account_result, host) :=
+        IHost.(Host.load_account_info_skip_cold_load) host address true skip_cold_load in
+      match account_result with
+      | Result.Ok account =>
+          (if account.(AccountInfoLoad.is_cold) then
+            gas_macro interpreter COLD_ACCOUNT_ACCESS_COST_ADDITIONAL
+              (fun interpreter => (None, interpreter, host)) (fun interpreter =>
+            (Some (account_info_load_original_bytes account), interpreter, host))
+          else
+            (Some (account_info_load_original_bytes account), interpreter, host))
+      | Result.Err LoadError.ColdLoadSkipped =>
+          (None, halt_oog interpreter, host)
+      | Result.Err LoadError.DBError =>
+          (None, halt_fatal interpreter, host)
+      end)
+    else
+      let gas := if Impl_SpecId.is_enabled_in spec_id SpecId.TANGERINE then 700 else 20 in
+      gas_macro interpreter gas
+        (fun interpreter => (None, interpreter, host)) (fun interpreter =>
+      let '(code_opt, host) := IHost.(Host.load_account_code) host address in
+      match code_opt with
+      | Some code => (Some code.(StateLoad.data), interpreter, host)
+      | None => (None, halt_fatal interpreter, host)
+      end) in
+  let '(code_opt, interpreter, host) := get_code interpreter host in
+  match code_opt with
+  | None => (interpreter, host)
+  | Some code =>
   let code_len := Impl_Bytes.len code.(Bytes.value) in
   let code_offset := Z.min (i[as_usize_saturated_macro code_offset] mod 2^64) i[code_len] in
-  resize_memory_macro interpreter memory_offset len
-    (fun interpreter => (interpreter, host)) (fun interpreter =>
-
   let memory :=
     IInterpreterTypes.(InterpreterTypes.MemoryTrait_for_Memory).(MemoryTrait.set_data)
       interpreter.(Interpreter.memory)
-      memory_offset
+      memory_offset_usize
       code_offset
       len
       code.(Bytes.value).(bytes.Bytes.value) in
   (interpreter <| Interpreter.memory := memory |>, host)
-  )))) end).
+  end))).
 
 Lemma extcodecopy_eq
     {WIRE H : Set} `{Link WIRE} `{Link H}
@@ -101,4 +141,26 @@ Lemma extcodecopy_eq
     )
   }}.
 Proof.
+  with_strategy transparent [run_extcodecopy] unfold extcodecopy, run_extcodecopy; cbn.
+  popn_macro_eq InterpreterTypesEq.
+  match goal with
+  | array : array.t _ _ |- _ =>
+    destruct array as [[address [memory_offset [code_offset [len []]]]]]
+  end.
+  s. {
+    apply Impl_IntoAddress_for_U256.into_address_eq.
+  }
+  s. {
+    apply InterpreterTypesEq.
+  }
+  as_usize_or_fail_macro_eq InterpreterTypesEq.
+  s. {
+    apply calc.copy_cost_eq.
+  }
+  s. {
+    apply Impl_u64.max_eq.
+  }
+  gas_macro_eq idtac.
+  s.
+  destruct ((len.(lib.Uint.value) mod 2 ^ 64) mod 2 ^ 64 =? 0) eqn:?; cbn.
 Admitted.
